Move OWGCounter to SteelSel

examples/steel/OWGCounter.fst
@@ -33,17 +33,17 @@ module G = FStar.Ghost
 
 open Steel.Memory
 open Steel.FractionalPermission
-open Steel.Reference
-open Steel.SpinLock
+open Steel.SelReference
+open Steel.SelSpinLock
 
-open Steel.Effect.Atomic
-open Steel.Effect
+open Steel.SelEffect.Atomic
+open Steel.SelEffect
 
-module R = Steel.Reference
+module R = Steel.SelReference
 module P = Steel.FractionalPermission
-module A = Steel.Effect.Atomic
+module A = Steel.SelEffect.Atomic
 
-#set-options "--using_facts_from '* -FStar.Tactics -FStar.Reflection' --fuel 0 --ifuel 0"
+#set-options "--ide_id_info_off --using_facts_from '* -FStar.Tactics -FStar.Reflection' --fuel 0 --ifuel 0"
 
 let half_perm = half_perm full_perm
 
@@ -64,62 +64,85 @@ let lock_inv_pred (r:ref int) (r1 r2:ghost_ref int) =
   fun (x:G.erased int & G.erased int) -> lock_inv_slprop r r1 r2 x
 
 [@@ __reduce__]
-let lock_inv (r:ref int) (r1 r2:ghost_ref int) : slprop =
+let lock_inv (r:ref int) (r1 r2:ghost_ref int) : vprop =
   h_exists (lock_inv_pred r r1 r2)
 
-#push-options "--warn_error -271"
+#push-options "--warn_error -271 --fuel 1 --ifuel 1"
 let lock_inv_equiv_lemma (r:ref int) (r1 r2:ghost_ref int)
   : Lemma (lock_inv r r1 r2 `equiv` lock_inv r r2 r1)
-  = let aux (r:ref int) (r1 r2:ghost_ref int) (m:mem)
+  =
+  let aux (r:ref int) (r1 r2:ghost_ref int) (m:mem)
       : Lemma
-          (requires interp (lock_inv r r1 r2) m)
-          (ensures interp (lock_inv r r2 r1) m)
+          (requires interp (hp_of (lock_inv r r1 r2)) m)
+          (ensures interp (hp_of (lock_inv r r2 r1)) m)
           [SMTPat ()]
-      = let w : G.erased (G.erased int & G.erased int) = id_elim_exists (lock_inv_pred r r1 r2) m in
+      = assert (
+          Steel.Memory.h_exists #(G.erased int & G.erased int) (fun x -> hp_of (lock_inv_pred r r1 r2 x)) ==
+          h_exists_sl #(G.erased int & G.erased int) (lock_inv_pred r r1 r2))
+          by (FStar.Tactics.norm [delta_only [`%h_exists_sl]]);
+
+        let w : G.erased (G.erased int & G.erased int) = id_elim_exists (fun x -> hp_of (lock_inv_pred r r1 r2 x)) m in
         assert ((ghost_pts_to r1 half_perm (snd (snd w, fst w)) `star`
                  ghost_pts_to r2 half_perm (fst (snd w, fst w)) `star`
                  pts_to r full_perm (G.hide (G.reveal (fst (snd w, fst w)) + G.reveal (snd (snd w, fst w))))) `equiv`
                 (ghost_pts_to r2 half_perm (fst (snd w, fst w)) `star`
                  ghost_pts_to r1 half_perm (snd (snd w, fst w)) `star`
-                 pts_to r full_perm (G.hide (G.reveal (fst (snd w, fst w)) + G.reveal (snd (snd w, fst w)))))) by Steel.Memory.Tactics.canon ();
+                 pts_to r full_perm (G.hide (G.reveal (fst (snd w, fst w)) + G.reveal (snd (snd w, fst w)))))) by (FStar.Tactics.norm [delta_attr [`%__steel_reduce__]]; canon' false (`true_p) (`true_p));
 
-        intro_h_exists (snd w, fst w) (lock_inv_pred r r2 r1) m in
-    ()
+        reveal_equiv
+          (ghost_pts_to r1 half_perm (snd (snd w, fst w)) `star`
+                 ghost_pts_to r2 half_perm (fst (snd w, fst w)) `star`
+                 pts_to r full_perm (G.hide (G.reveal (fst (snd w, fst w)) + G.reveal (snd (snd w, fst w)))))
+          (ghost_pts_to r2 half_perm (fst (snd w, fst w)) `star`
+                 ghost_pts_to r1 half_perm (snd (snd w, fst w)) `star`
+                 pts_to r full_perm (G.hide (G.reveal (fst (snd w, fst w)) + G.reveal (snd (snd w, fst w)))));
+
+        assert (interp (hp_of (lock_inv_pred r r2 r1 (snd w, fst w))) m);
+
+        intro_h_exists (snd w, fst w) (fun x -> hp_of (lock_inv_pred r r2 r1 x)) m;
+        assert (interp (Steel.Memory.h_exists (fun x -> hp_of (lock_inv_pred r r2 r1 x))) m);
+
+       assert (
+          Steel.Memory.h_exists #(G.erased int & G.erased int) (fun x -> hp_of (lock_inv_pred r r2 r1 x)) ==
+          h_exists_sl #(G.erased int & G.erased int) (lock_inv_pred r r2 r1))
+          by (FStar.Tactics.norm [delta_only [`%h_exists_sl]]) in
+
+  reveal_equiv (lock_inv r r1 r2) (lock_inv r r2 r1)
 #pop-options
 
 inline_for_extraction noextract
 let og_acquire (r:ref int) (r_mine r_other:ghost_ref int) (b:G.erased bool)
   (l:lock (lock_inv r (if b then r_mine else r_other)
                       (if b then r_other else r_mine)))
-  : SteelT unit
+  : SteelSelT unit
       emp
       (fun _ -> lock_inv r r_mine r_other)
   = acquire l;
     if b then begin
-      change_slprop (lock_inv r (if b then r_mine else r_other)
+      rewrite_slprop (lock_inv r (if b then r_mine else r_other)
                                 (if b then r_other else r_mine))
                     (lock_inv r r_mine r_other)
                     (fun _ -> ());
       ()
     end
     else begin
-      change_slprop (lock_inv r (if b then r_mine else r_other)
+      rewrite_slprop (lock_inv r (if b then r_mine else r_other)
                                 (if b then r_other else r_mine))
                     (lock_inv r r_other r_mine)
                     (fun _ -> ());
       lock_inv_equiv_lemma r r_other r_mine;
-      rewrite_context #_ #(lock_inv r r_other r_mine) #(lock_inv r r_mine r_other) ()
+      rewrite_slprop (lock_inv r r_other r_mine) (lock_inv r r_mine r_other) (fun _ -> reveal_equiv (lock_inv r r_other r_mine) (lock_inv r r_mine r_other))
     end
 
 inline_for_extraction noextract
 let og_release (r:ref int) (r_mine r_other:ghost_ref int) (b:G.erased bool)
   (l:lock (lock_inv r (if b then r_mine else r_other)
                       (if b then r_other else r_mine)))
-  : SteelT unit
+  : SteelSelT unit
       (lock_inv r r_mine r_other)
       (fun _ -> emp)
   = if b then begin
-      change_slprop (lock_inv r r_mine r_other)
+      rewrite_slprop (lock_inv r r_mine r_other)
                     (lock_inv r (if b then r_mine else r_other)
                                 (if b then r_other else r_mine))
                     (fun _ -> ());
@@ -127,8 +150,8 @@ let og_release (r:ref int) (r_mine r_other:ghost_ref int) (b:G.erased bool)
     end
     else begin
       lock_inv_equiv_lemma r r_mine r_other;
-      rewrite_context #_ #(lock_inv r r_mine r_other) #(lock_inv r r_other r_mine) ();
-      change_slprop (lock_inv r r_other r_mine)
+      rewrite_slprop (lock_inv r r_mine r_other) (lock_inv r r_other r_mine) (fun _ -> reveal_equiv (lock_inv r r_mine r_other) (lock_inv r r_other r_mine));
+      rewrite_slprop (lock_inv r r_other r_mine)
                     (lock_inv r (if b then r_mine else r_other)
                                 (if b then r_other else r_mine))
                     (fun _ -> ())
@@ -142,40 +165,40 @@ let g_incr (n:G.erased int) = G.elift1 (fun (n:int) -> n + 1) n
 
 inline_for_extraction noextract
 let incr_ctr (#v:G.erased int) (r:ref int)
-  : SteelT unit
+  : SteelSelT unit
       (pts_to r full_perm v)
       (fun _ -> pts_to r full_perm (g_incr v))
-  = let n = R.read r in
-    R.write r (n+1);
-    A.change_slprop (pts_to r full_perm (n + 1))
+  = let n = R.read_pt r in
+    R.write_pt r (n+1);
+    rewrite_slprop (pts_to r full_perm (n + 1))
                   (pts_to r full_perm (g_incr v))
                   (fun _ -> ())
 
 inline_for_extraction noextract
 let rewrite_perm(#a:Type) (#v:G.erased a) (r:ghost_ref a) (p1 p2:P.perm)
-  : Steel unit
+  : SteelSel unit
       (ghost_pts_to r p1 v)
       (fun _ -> ghost_pts_to r p2 v)
       (fun _ -> p1 == p2)
       (fun _ _ _ -> True)
-  = change_slprop (ghost_pts_to r p1 v)
+  = rewrite_slprop (ghost_pts_to r p1 v)
                   (ghost_pts_to r p2 v)
                   (fun _ -> ())
 
 inline_for_extraction noextract
 let incr_ghost_contrib (#v1 #v2:G.erased int) (r:ghost_ref int)
-  : Steel unit
+  : SteelSel unit
       (ghost_pts_to r half_perm v1 `star`
        ghost_pts_to r half_perm v2)
       (fun _ -> ghost_pts_to r half_perm (g_incr v1) `star`
              ghost_pts_to r half_perm (g_incr v2))
       (fun _ -> True)
       (fun _ _ _ -> v1 == v2)
-  = ghost_gather #_ #_ #half_perm #half_perm #v1 #v2 r;
+  = ghost_gather_pt #_ #_ #half_perm #half_perm #v1 #v2 r;
     rewrite_perm r (sum_perm half_perm half_perm) full_perm;
-    ghost_write r (g_incr v1);
-    ghost_share r;
-    change_slprop (ghost_pts_to r (P.half_perm P.full_perm) (g_incr v1) `star`
+    ghost_write_pt r (g_incr v1);
+    ghost_share_pt r;
+    rewrite_slprop (ghost_pts_to r (P.half_perm P.full_perm) (g_incr v1) `star`
                    ghost_pts_to r (P.half_perm P.full_perm) (g_incr v1))
                   (ghost_pts_to r half_perm (g_incr v1) `star`
                    ghost_pts_to r half_perm (g_incr v2))
@@ -186,37 +209,37 @@ let incr (r:ref int) (r_mine r_other:ghost_ref int) (b:G.erased bool)
                       (if b then r_other else r_mine)))
   (n_ghost:G.erased int)
   ()
-  : SteelT unit
+  : SteelSelT unit
       (ghost_pts_to r_mine half_perm n_ghost)
       (fun _ -> ghost_pts_to r_mine half_perm (g_incr n_ghost))
   = og_acquire r r_mine r_other b l;
-    let w : G.erased (G.erased int & G.erased int) = witness_h_exists () in
+    let w : G.erased (G.erased int & G.erased int) = witness_exists () in
     incr_ctr r;
     incr_ghost_contrib #n_ghost #(fst w) r_mine;
-    change_slprop (pts_to r full_perm (g_incr (G.hide (fst w + snd w))))
+    rewrite_slprop (pts_to r full_perm (g_incr (G.hide (fst w + snd w))))
                   (pts_to r full_perm (G.hide (g_incr (fst w) + snd w)))
                   (fun _ -> ());
     intro_exists (g_incr (fst w), snd w) (lock_inv_pred r r_mine r_other);
     og_release r r_mine r_other b l
 
 let incr_main (#v:G.erased int) (r:ref int)
-  : SteelT unit
+  : SteelSelT unit
       (pts_to r full_perm v)
       (fun _ -> pts_to r full_perm (G.hide (G.reveal v + 2)))
   = //allocate the two contribution references
-    let r1 = ghost_alloc (G.hide 0) in
-    let r2 = ghost_alloc v in
+    let r1 = ghost_alloc_pt (G.hide 0) in
+    let r2 = ghost_alloc_pt v in
 
     //split their permissions into half
-    ghost_share r1;
-    change_slprop (ghost_pts_to r1 (P.half_perm P.full_perm) (G.hide 0) `star`
+    ghost_share_pt r1;
+    rewrite_slprop (ghost_pts_to r1 (P.half_perm P.full_perm) (G.hide 0) `star`
                    ghost_pts_to r1 (P.half_perm P.full_perm) (G.hide 0))
                   (ghost_pts_to r1 half_perm (G.hide 0) `star`
                    ghost_pts_to r1 half_perm (G.hide 0))
                   (fun _ -> ());
 
-    ghost_share r2;
-    change_slprop (ghost_pts_to r2 (P.half_perm P.full_perm) v `star`
+    ghost_share_pt r2;
+    rewrite_slprop (ghost_pts_to r2 (P.half_perm P.full_perm) v `star`
                    ghost_pts_to r2 (P.half_perm P.full_perm) v)
                   (ghost_pts_to r2 half_perm v `star`
                    ghost_pts_to r2 half_perm v)
@@ -224,7 +247,7 @@ let incr_main (#v:G.erased int) (r:ref int)
 
 
     //rewrite the value of `r` to bring it in the shape as expected by the lock
-    change_slprop (pts_to r full_perm v)
+    rewrite_slprop (pts_to r full_perm v)
                   (pts_to r full_perm (G.hide (G.reveal (fst (G.hide 0, v)) + G.reveal (snd (G.hide 0, v)))))
                   (fun _ -> ());
 
@@ -239,14 +262,14 @@ let incr_main (#v:G.erased int) (r:ref int)
     //take the lock
     acquire l;
 
-    let w = A.witness_h_exists () in
+    let w = witness_exists () in
 
     //gather the permissions for the ghost references, and then drop them
-    ghost_gather #_ #_ #_ #_ #(fst w) #_ r1;
-    ghost_gather #_ #_ #_ #_ #(snd w) #_ r2;
+    ghost_gather_pt #_ #_ #_ #_ #(fst w) #_ r1;
+    ghost_gather_pt #_ #_ #_ #_ #(snd w) #_ r2;
     drop (ghost_pts_to r1 (P.sum_perm half_perm half_perm) (fst w));
     drop (ghost_pts_to r2 (P.sum_perm half_perm half_perm) (snd w));
 
-    change_slprop (pts_to r full_perm (G.hide (G.reveal (fst w) + G.reveal (snd w))))
+    rewrite_slprop (pts_to r full_perm (G.hide (G.reveal (fst w) + G.reveal (snd w))))
                   (pts_to r full_perm (v + 2))
                   (fun _ -> ())
